Spec.ECIES using DH, AEAD, Hash agile modules

specs/Spec.ECIES.fst
@@ -7,6 +7,8 @@ open Lib.Sequence
 open Lib.ByteSequence
 
 
+module DH = Spec.DH
+module AEAD = Spec.AEAD
 module Hash = Spec.Hash
 
 
@@ -19,27 +21,30 @@ let pow2_35_less_than_pow2_125 : _:unit{pow2 32 * pow2 3 <= pow2 125 - 1} = asse
 
 #set-options "--z3rlimit 100"
 
-type ciphersuite =
-  | Curve25519_AES128_GCM_SHA2_256
-  | Curve25519_AES128_GCM_SHA2_512
-  | Curve448_AES128_GCM_SHA2_256
-  | Curve448_AES128_GCM_SHA2_512
+/// Types
 
-(** Ciphersuite identifiers *)
+type ciphersuite = DH.algorithm & AEAD.algorithm & a:Hash.algorithm{a == Hash.SHA2_256 \/ a == Hash.SHA2_512}
+
 val id_of_cs: cs:ciphersuite -> Tot (lbytes 1)
 let id_of_cs cs =
   match cs with
-  | Curve25519_AES128_GCM_SHA2_256 -> create 1 (u8 0)
-  | Curve25519_AES128_GCM_SHA2_512 -> create 1 (u8 1)
-  | Curve448_AES128_GCM_SHA2_256 -> create 1 (u8 2)
-  | Curve448_AES128_GCM_SHA2_512 -> create 1 (u8 3)
+  | DH.DH_Curve25519, AEAD.AEAD_AES128_GCM,        Hash.SHA2_256 -> create 1 (u8 0)
+  | DH.DH_Curve25519, AEAD.AEAD_AES128_GCM,        Hash.SHA2_512 -> create 1 (u8 1)
+  | DH.DH_Curve25519, AEAD.AEAD_Chacha20_Poly1305, Hash.SHA2_256 -> create 1 (u8 2)
+  | DH.DH_Curve25519, AEAD.AEAD_Chacha20_Poly1305, Hash.SHA2_512 -> create 1 (u8 3)
+  | DH.DH_Curve448,   AEAD.AEAD_AES128_GCM,        Hash.SHA2_256 -> create 1 (u8 4)
+  | DH.DH_Curve448,   AEAD.AEAD_AES128_GCM,        Hash.SHA2_512 -> create 1 (u8 5)
+  | DH.DH_Curve448,   AEAD.AEAD_Chacha20_Poly1305, Hash.SHA2_256 -> create 1 (u8 6)
+  | DH.DH_Curve448,   AEAD.AEAD_Chacha20_Poly1305, Hash.SHA2_512 -> create 1 (u8 7)
 
-let hash_of_cs (cs:ciphersuite) : Spec.Hash.algorithm =
-  match cs with
-  | Curve25519_AES128_GCM_SHA2_256 -> Hash.SHA2_256
-  | Curve25519_AES128_GCM_SHA2_512 -> Hash.SHA2_512
-  | Curve448_AES128_GCM_SHA2_256 -> Hash.SHA2_256
-  | Curve448_AES128_GCM_SHA2_512 -> Hash.SHA2_512
+let curve_of_cs (cs:ciphersuite) : DH.algorithm =
+  let (c,a,h) = cs in c
+
+let aead_of_cs (cs:ciphersuite) : AEAD.algorithm =
+  let (c,a,h) = cs in a
+
+let hash_of_cs (cs:ciphersuite) : Hash.algorithm =
+  let (c,a,h) = cs in h
 
 
 /// Constants
@@ -61,101 +66,76 @@ let const_label_key : lbytes 9 =
 /// Constants sizes
 
 inline_for_extraction let vsize_nonce: size_nat = 12 (* AES_GCM with TLS length IV *)
-inline_for_extraction let vsize_key_symmetric (cs:ciphersuite): size_nat = 16 + 8
-inline_for_extraction let vsize_key_asymmetric (cs:ciphersuite): size_nat =
-  match cs with
-  | Curve25519_AES128_GCM_SHA2_256 -> 32
-  | Curve25519_AES128_GCM_SHA2_512 -> 32
-  | Curve448_AES128_GCM_SHA2_256 -> 56
-  | Curve448_AES128_GCM_SHA2_512 -> 56
-
+inline_for_extraction let vsize_key (cs:ciphersuite): size_nat = AEAD.size_key (aead_of_cs cs) + 8
+inline_for_extraction let vsize_key_asymmetric (cs:ciphersuite): size_nat = DH.size_key (curve_of_cs cs)
 
 /// Types
 
 type key_public_s (cs:ciphersuite) = lbytes (vsize_key_asymmetric cs)
 type key_private_s (cs:ciphersuite) = lbytes (vsize_key_asymmetric cs)
-type key_s (cs:ciphersuite) = lbytes (vsize_key_symmetric cs)
+type key_s (cs:ciphersuite) = lbytes (vsize_key cs)
 
 
 /// Cryptographic Primitives
-
-val dh: cs:ciphersuite -> key_private_s cs -> key_public_s cs -> Tot (option (lbytes (vsize_key_asymmetric cs)))
-let dh cs kpriv kpub =
-  let secret =
-    match cs with
-    | Curve25519_AES128_GCM_SHA2_256
-    | Curve25519_AES128_GCM_SHA2_512 -> Curve25519.scalarmult kpriv kpub
-    | Curve448_AES128_GCM_SHA2_256
-    | Curve448_AES128_GCM_SHA2_512 -> Curve448.scalarmult kpriv kpub
-  in
-  let unsafe : bool = for_all (fun a -> uint_to_nat #U8 a = 0) secret in
-  if unsafe then None else Some secret
-
-
-val secret_to_public: cs:ciphersuite -> key_private_s cs -> Tot (option (key_public_s cs))
-let secret_to_public cs kpriv =
-  let basepoint_zeros = create (vsize_key_asymmetric cs) (u8 0) in
-  let basepoint = upd basepoint_zeros ((vsize_key_asymmetric cs) - 1) (u8 0x09) in
-  dh cs kpriv basepoint
-
 
 val encap: cs:ciphersuite -> kpub:key_public_s cs -> Tot (option (key_s cs & key_public_s cs))
 let encap cs kpub =
   match crypto_random (vsize_key_asymmetric cs) with
   | None -> None
   | Some eph_kpriv ->
-  match secret_to_public cs eph_kpriv with
-  | None -> None
-  | Some eph_kpub ->
-  match dh cs eph_kpriv kpub with
-  | None -> None
-  | Some secret ->
-    let salt = (id_of_cs cs) @| eph_kpub @| kpub in
-    let extracted = Spec.HKDF.hkdf_extract (hash_of_cs cs) salt secret in
-    let key = Spec.HKDF.hkdf_expand (hash_of_cs cs) extracted const_label_key (vsize_key_symmetric cs) in
-    Some (key, eph_kpub)
+    let eph_kpub = DH.secret_to_public (curve_of_cs cs) eph_kpriv in
+    match DH.dh (curve_of_cs cs) eph_kpriv kpub with
+    | None -> None
+    | Some secret ->
+      let salt = (id_of_cs cs) @| eph_kpub @| kpub in
+      let extracted = Spec.HKDF.hkdf_extract (hash_of_cs cs) salt secret in
+      let key = Spec.HKDF.hkdf_expand (hash_of_cs cs) extracted const_label_key (vsize_key cs) in
+      Some (key, eph_kpub)
 
 
 val decap: cs:ciphersuite -> key_private_s cs -> eph_kpub:key_public_s cs -> Tot (option (key_s cs))
 let decap cs kpriv eph_kpub =
-  match secret_to_public cs kpriv with
-  | None -> None
-  | Some kpub ->
-  match dh cs kpriv eph_kpub with
+  let kpub = DH.secret_to_public (curve_of_cs cs) kpriv in
+  match DH.dh (curve_of_cs cs) kpriv eph_kpub with
   | None -> None
   | Some secret ->
     let salt = (id_of_cs cs) @| eph_kpub @| kpub in
     let extracted = Spec.HKDF.hkdf_extract (hash_of_cs cs) salt secret in
-    let key = Spec.HKDF.hkdf_expand (hash_of_cs cs) extracted const_label_key (vsize_key_symmetric cs) in
+    let key = Spec.HKDF.hkdf_expand (hash_of_cs cs) extracted const_label_key (vsize_key cs) in
     Some key
 
 
 val encrypt:
     cs: ciphersuite
   -> sk: key_s cs
-  -> input: bytes{length input + 16 <= max_size_t}
-  -> aad: bytes{length aad + 16 <= max_size_t}
+  -> input: bytes{length input <= max_size_t
+           /\ length input + AEAD.size_block (aead_of_cs cs) <= max_size_t
+           /\ length input + AEAD.padlen (aead_of_cs cs) (length input) <= max_size_t}
+  -> aad: bytes {length aad <= max_size_t /\ length aad + AEAD.padlen (aead_of_cs cs) (length aad) <= max_size_t}
   -> counter: uint32 ->
   Tot bytes
 
 let encrypt cs sk input aad counter =
-  let key = sub sk 0 16 in
-  let nonce = sub sk 16 8 in
+  let klen = AEAD.size_key (aead_of_cs cs) in
+  let key = sub sk 0 klen in
+  let nonce = sub sk klen 8 in
   let ctr = uint_to_bytes_le counter in
-  Spec.AES128_GCM.aead_encrypt key (nonce @| ctr) input aad
+  AEAD.aead_encrypt (aead_of_cs cs) key (nonce @| ctr) input aad
 
 
 val decrypt:
     cs: ciphersuite
   -> sk: key_s cs
-  -> input:bytes{16 <= length input /\ length input <= max_size_t}
-  -> aad:bytes{length aad + 16 <= max_size_t}
+  -> c: bytes{AEAD.size_tag (aead_of_cs cs) <= length c /\ length c <= max_size_t}
+  -> aad: bytes{length aad <= max_size_t
+             /\ (length c + length aad) / 64 <= max_size_t
+             /\ length aad + AEAD.padlen (aead_of_cs cs) (length aad) <= max_size_t}
   -> counter:uint32 ->
-  Tot bytes
+  Tot (option (lbytes (length c - AEAD.size_tag (aead_of_cs cs))))
 
 let decrypt cs sk input aad counter =
-  let key = sub sk 0 16 in
-  let nonce = sub sk 16 8 in
+  let klen = AEAD.size_key (aead_of_cs cs) in
+  let key = sub sk 0 klen in
+  let nonce = sub sk klen 8 in
   let ctr = uint_to_bytes_le counter in
-  Spec.AES128_GCM.aead_decrypt key (nonce @| ctr) input aad
-
+  AEAD.aead_decrypt (aead_of_cs cs) key (nonce @| ctr) input aad
